2
========================================================

$$
p_k(x) = \frac {\pi_k
                \frac {1} {\sqrt{2 \pi} \sigma}
                \exp(- \frac {1} {2 \sigma^2} (x - \mu_k)^2)
               }
               {\sum {
                \pi_l
                \frac {1} {\sqrt{2 \pi} \sigma}
                \exp(- \frac {1} {2 \sigma^2} (x - \mu_l)^2)
               }}
$$

$\frac {1} {\sqrt{2 \pi} \sigma}$ cancels out.

$$
p_k(x) = \frac {\pi_k
                \exp(- \frac {1} {2 \sigma^2} (x - \mu_k)^2)
               }
               {\sum {
                \pi_l
                \exp(- \frac {1} {2 \sigma^2} (x - \mu_l)^2)
               }}
\\
       = \frac {\pi_k
                \exp(- \frac {1} {2 \sigma^2} (x^2 - 2\mu_k x  + \mu_k^2))
               }
               {\sum {
                \pi_l
                \exp(- \frac {1} {2 \sigma^2} (x^2 - 2\mu_l x + \mu_l^2))
               }}
$$

$x^2$ cancels out.

$$
p_k(x) = \frac {\pi_k
                \exp(\frac {1} {2 \sigma^2} (2\mu_k x - \mu_k^2))
               }
               {\sum {
                \pi_l
                \exp(\frac {1} {2 \sigma^2} (2\mu_l x - \mu_l^2))
               }}
\\
\log(p_k(x)) = \frac {\log(\pi_k) +
                      \frac {1} {2 \sigma^2} (2\mu_k x - \mu_k^2)
                     }
                     {\log(\sum {
                      \pi_l
                      \exp(\frac {1} {2 \sigma^2} (2\mu_l x - \mu_l^2))
                     })}
\\
\log(p_k(x)) 
\log(\sum {\pi_l \exp(\frac {1} {2 \sigma^2} (2\mu_l x - \mu_l^2))})
= \log(\pi_k) + \frac {1} {2 \sigma^2} (2\mu_k x - \mu_k^2)
\\
\delta_k(x) = x \frac {\mu_k} {\sigma^2} - \frac {\mu_k^2} {2 \sigma^2}
              + \log(\pi_k)
$$