7
========================================================
$$
p_k(x) = \frac {\pi_k
                \frac {1} {\sqrt{2 \pi} \sigma}
                \exp(- \frac {1} {2 \sigma^2} (x - \mu_k)^2)
               }
               {\sum {
                \pi_l
                \frac {1} {\sqrt{2 \pi} \sigma}
                \exp(- \frac {1} {2 \sigma^2} (x - \mu_l)^2)
               }}
\\
       = \frac {\pi_{yes}
                \exp(- \frac {1} {2 \sigma^2}  (x - \mu_{yes})^2)
               }
               {\sum {
                \pi_l
                \exp(- \frac {1} {2 \sigma^2} (x - \mu_l)^2)
               }}
\\
       = \frac {\pi_{yes} \exp(- \frac {1} {2 \sigma^2}  (x - \mu_{yes})^2)}
               {
                \pi_{yes} \exp(- \frac {1} {2 \sigma^2} (x - \mu_{yes})^2) +
                \pi_{no}  \exp(- \frac {1} {2 \sigma^2}  (x - \mu_{no})^2)
               }
\\
       = \frac {0.80 \exp(- \frac {1} {2 * 36}  (x - 10)^2)}
               {
                0.80 \exp(- \frac {1} {2 * 36} (x - 10)^2) +
                0.20 \exp(- \frac {1} {2 * 36}  x^2)
               }
\\
p_{yes}(4)  = \frac {0.80 \exp(- \frac {1} {2 * 36}  (4 - 10)^2)}
               {
                0.80 \exp(- \frac {1} {2 * 36} (4 - 10)^2) +
                0.20 \exp(- \frac {1} {2 * 36}  4^2)
               }
        = 75.2\%
$$
